Semantics/Imp/Denotational.lean
@@ -24,20 +24,18 @@ theorem monotone_denote_loop: monotone (denote_loop b c) :=
 
 notation (priority := high) "⟦" c "⟧" => denote c
 
--- #simp (σ₀, σ₀⟪"x"≔5⟫⟪"x"≔1⟫) ∈ ⟦⦃x = 5; if x <= 1 {skip} else {x = 1}⦄⟧
--- #simp (σ₀, σ₀⟪"x"≔5⟫) ∈ ⟦⦃x = 5; while x <= 1 {x = 1}⦄⟧
+#check (σ₀, σ₀⟪"x"≔5⟫⟪"x"≔1⟫) ∈ ⟦⦃x = 5; if x <= 1 then skip else x = 1 end⦄⟧
+#check (σ₀, σ₀⟪"x"≔5⟫) ∈ ⟦⦃x = 5; while x <= 1 loop x = 1 end⦄⟧
 
 namespace denote
 
-
-@[simp]
 instance equiv: Setoid Com := ⟨(⟦·⟧ = ⟦·⟧), ⟨(Eq.refl ⟦.⟧), Eq.symm, Eq.trans⟩⟩
 
 theorem skipl: (skip₁;;c) ≈ c :=
-  by simp [HasEquiv.Equiv, denote, SRel.comp_id_left]
+  by simp only [HasEquiv.Equiv, equiv, denote, SRel.comp_id_left]
 
 theorem skipr: (c;;skip₁) ≈ c :=
-  by simp [HasEquiv.Equiv, denote, SRel.comp_id_right]
+  by simp only [HasEquiv.Equiv, equiv, denote, SRel.comp_id_right]
 
 theorem while_unfold:
   while b loop c end ≈ if b then c;; while b loop c end else skip₁ end :=
@@ -49,17 +47,17 @@ theorem while_unfold:
 
 theorem cat_congr (hc: c₁ ≈ c₂) (hd: d₁ ≈ d₂):
   (c₁;;d₁) ≈ (c₂;;d₂) := by
-  simp [HasEquiv.Equiv, denote]
+  simp only [HasEquiv.Equiv, equiv, denote]
   exact hc ▸ hd ▸ rfl
 
 theorem cond_congr (hc: c1 ≈ c2) (hd: d1 ≈ d2):
   if b then c1 else d1 end ≈ if b then c2 else d2 end := by
-  simp [HasEquiv.Equiv, denote]
+  simp only [HasEquiv.Equiv, equiv, denote]
   exact hc ▸ hd ▸ rfl
 
 theorem loop_congr (hc: c1 ≈ c2):
   while b loop c1 end ≈ while b loop c2 end := by
-  simp [HasEquiv.Equiv, denote]
+  simp only [HasEquiv.Equiv, equiv, denote]
   exact hc ▸ rfl
 
 end denote
